feat(IR): support dialect-local setProperties

UnitTest/Dialect.lean
@@ -29,12 +29,6 @@ abbrev Veir.Arith.from? (op : OpInfo) [HasOpInfo OpInfo] [HasDialect OpInfo Arit
 #guard Arith.from? (Arith.addi : OpCode) = some Arith.addi
 #guard Arith.from? (OpCode.builtin .module) = none
 
-def Veir.OperationPtr.setProperties!' {OpInfo Dialect : Type} [HasOpInfo OpInfo]
-    [HasDialectOpInfo Dialect] [HasDialect OpInfo Dialect]
-    (op : OperationPtr) (ctx : WfIRContext OpInfo) (opCode : Dialect)
-    (props : HasDialectOpInfo.propertiesOf opCode) : WfIRContext OpInfo :=
-  WfRewriter.setProperties! ctx op (HasDialect.ofDialectProperties OpInfo opCode props)
-
 /--
 A minimal pass that can be instantiated for any ambient opcode type containing
 the Arith dialect. It exercises both opcode projection and property transport.
@@ -47,12 +41,10 @@ private def genericArithAwarePass {OpInfo : Type} [HasOpInfo OpInfo]
     /- Matching an `arith` operation, here an `addi`. -/
     let some .addi := Arith.from? (op.getOpType! ctx.raw) | return ctx
     /- Getting the property of an operation with a type based on the dialect. -/
-    let _a := op.getProperties! ctx.raw Arith.addi
-    /- Check that we automatically derive the correct properties type. -/
-    let _b : ArithIntegerOverflowFlagsProperties := _a
-    /- Create -/
-    let ctx := op.setProperties!' ctx Arith.addi
-      (ArithIntegerOverflowFlagsProperties.mk { nsw := true, nuw := false })
+    let _a : ArithIntegerOverflowFlagsProperties := op.getProperties! ctx.raw Arith.addi
+    /- Set dialect-local properties. -/
+    let props := ArithIntegerOverflowFlagsProperties.mk { nsw := true, nuw := false }
+    let ctx := WfRewriter.setProperties! (Dialect := Arith) ctx op Arith.addi props
     return ctx
 
 example : Pass OpCode := genericArithAwarePass
