Veir/PatternRewriter/Basic.lean
@@ -215,13 +215,14 @@ def insertOp! (rewriter: PatternRewriter OpInfo) (op: OperationPtr) (ip : Insert
 /--
 Set the properties of an operation in place, and re-enqueue it.
 -/
-def setProperties (rewriter: PatternRewriter OpInfo) (op: OperationPtr) (opCode : OpInfo)
-    (newProps : HasOpInfo.propertiesOf opCode)
+def setProperties {Dialect : Type} [HasDialectOpInfo Dialect] [HasDialect OpInfo Dialect]
+    (rewriter: PatternRewriter OpInfo) (op: OperationPtr) (opCode : Dialect)
+    (newProps : HasDialectOpInfo.propertiesOf opCode)
     (opIn : op.InBounds rewriter.ctx.raw := by grind)
     (hprop : op.getOpType! rewriter.ctx.raw = opCode := by grind)
     : PatternRewriter OpInfo :=
   { rewriter with
-    ctx := WfRewriter.setProperties rewriter.ctx op newProps (by grind) (by grind),
+    ctx := WfRewriter.setProperties rewriter.ctx op opCode newProps opIn hprop,
     hasDoneAction := true,
     worklist := rewriter.worklist.push op,
   }
@@ -230,8 +231,9 @@ def setProperties (rewriter: PatternRewriter OpInfo) (op: OperationPtr) (opCode 
 Set the properties of an operation in place, panicking if the operation is out of bounds, or if
 the property types don't match.
 -/
-def setProperties! (rewriter: PatternRewriter OpInfo) (op: OperationPtr) (opCode : OpInfo)
-    (newProps : HasOpInfo.propertiesOf opCode) : PatternRewriter OpInfo :=
+def setProperties! {Dialect : Type} [HasDialectOpInfo Dialect] [HasDialect OpInfo Dialect]
+    (rewriter: PatternRewriter OpInfo) (op: OperationPtr) (opCode : Dialect)
+    (newProps : HasDialectOpInfo.propertiesOf opCode) : PatternRewriter OpInfo :=
   if opIn : op.InBounds rewriter.ctx.raw then
     if hprop : op.getOpType! rewriter.ctx.raw = opCode then
       rewriter.setProperties op opCode newProps opIn hprop
