Veir/Rewriter/GetSet/Operation.lean
@@ -276,227 +276,235 @@ end Rewriter.setAttributes
 
 section Rewriter.setProperties
 
-variable {opCode: OpInfo} {op : OperationPtr} {newProps : HasOpInfo.propertiesOf opCode} {opIn : op.InBounds ctx}
-         {opIn: op.InBounds ctx} {hprop : op.getOpType! ctx = opCode}
+variable {op : OperationPtr} {newProps : HasDialectOpInfo.propertiesOf opCode}
+         {opIn : op.InBounds ctx} {hprop : op.getOpType! ctx = opCode}
 
 attribute [local grind] Rewriter.setProperties
 
 @[simp, grind =]
 theorem BlockPtr.get!_setProperties {block : BlockPtr} :
-    block.get! (Rewriter.setProperties ctx op newProps opIn hprop) =
+    block.get! (Rewriter.setProperties ctx op opCode newProps opIn hprop) =
     block.get! ctx := by
   grind
 
 @[simp, grind =]
 theorem BlockPtr.firstUse!_setProperties {block : BlockPtr} :
-    (block.get! (Rewriter.setProperties ctx op newProps opIn hprop)).firstUse =
+    (block.get! (Rewriter.setProperties ctx op opCode newProps opIn hprop)).firstUse =
     (block.get! ctx).firstUse := by
   grind
 
 @[simp, grind =]
 theorem BlockPtr.prev!_setProperties {block : BlockPtr} :
-    (block.get! (Rewriter.setProperties ctx op newProps opIn hprop)).prev =
+    (block.get! (Rewriter.setProperties ctx op opCode newProps opIn hprop)).prev =
     (block.get! ctx).prev := by
   grind
 
 @[simp, grind =]
 theorem BlockPtr.next!_setProperties {block : BlockPtr} :
-    (block.get! (Rewriter.setProperties ctx op newProps opIn hprop)).next =
+    (block.get! (Rewriter.setProperties ctx op opCode newProps opIn hprop)).next =
     (block.get! ctx).next := by
   grind
 
 @[simp, grind =]
 theorem BlockPtr.parent!_setProperties {block : BlockPtr} :
-    (block.get! (Rewriter.setProperties ctx op newProps opIn hprop)).parent =
+    (block.get! (Rewriter.setProperties ctx op opCode newProps opIn hprop)).parent =
     (block.get! ctx).parent := by
   grind
 
 @[simp, grind =]
 theorem BlockPtr.firstOp!_setProperties {block : BlockPtr} :
-    (block.get! (Rewriter.setProperties ctx op newProps opIn hprop)).firstOp =
+    (block.get! (Rewriter.setProperties ctx op opCode newProps opIn hprop)).firstOp =
     (block.get! ctx).firstOp := by
   grind
 
 @[simp, grind =]
 theorem BlockPtr.lastOp!_setProperties {block : BlockPtr} :
-    (block.get! (Rewriter.setProperties ctx op newProps opIn hprop)).lastOp =
+    (block.get! (Rewriter.setProperties ctx op opCode newProps opIn hprop)).lastOp =
     (block.get! ctx).lastOp := by
   grind
 
 @[grind =]
 theorem OperationPtr.get!_setProperties {operation : OperationPtr} :
-    operation.get! (Rewriter.setProperties ctx op newProps opIn hprop) =
+    operation.get! (Rewriter.setProperties ctx op opCode newProps opIn hprop) =
     if operation = op then
-      { operation.get! ctx with opType := op.getOpType! ctx, properties := hprop ▸ newProps }
+      { operation.get! ctx with
+        opType := op.getOpType! ctx
+        properties := hprop ▸ HasDialect.ofDialectProperties OpInfo opCode newProps }
     else
       operation.get! ctx := by
   grind
 
 @[simp, grind =]
 theorem OperationPtr.prev!_setProperties {op' : OperationPtr} :
-    (op'.get! (Rewriter.setProperties ctx op newProps opIn)).prev =
+    (op'.get! (Rewriter.setProperties ctx op opCode newProps opIn)).prev =
     (op'.get! ctx).prev := by
   grind
 
 @[simp, grind =]
 theorem OperationPtr.next!_setProperties {op' : OperationPtr} :
-    (op'.get! (Rewriter.setProperties ctx op newProps opIn)).next =
+    (op'.get! (Rewriter.setProperties ctx op opCode newProps opIn)).next =
     (op'.get! ctx).next := by
   grind
 
 @[simp, grind =]
 theorem OperationPtr.parent!_setProperties {op' : OperationPtr} :
-    (op'.get! (Rewriter.setProperties ctx op newProps opIn)).parent =
+    (op'.get! (Rewriter.setProperties ctx op opCode newProps opIn)).parent =
     (op'.get! ctx).parent := by
   grind
 
 @[simp, grind =]
 theorem OperationPtr.getOpType!_setProperties {op' : OperationPtr} :
-    op'.getOpType! (Rewriter.setProperties ctx op newProps opIn) =
+    op'.getOpType! (Rewriter.setProperties ctx op opCode newProps opIn) =
     op'.getOpType! ctx := by
   grind
 
 @[simp ,grind =]
 theorem OperationPtr.attrs!_setProperties {op' : OperationPtr} :
-    (op'.get! (Rewriter.setProperties ctx op newProps opIn)).attrs =
+    (op'.get! (Rewriter.setProperties ctx op opCode newProps opIn)).attrs =
     (op'.get! ctx).attrs := by
   grind
 
 @[grind =]
 theorem OperationPtr.getProperties!_setProperties
-    {op' : OperationPtr} {getterOpCode : Dialect} :
-    op'.getProperties! (Rewriter.setProperties ctx op newProps opIn hprop) getterOpCode =
+    {GetterDialect : Type} [HasDialectOpInfo GetterDialect]
+    [HasDialect OpInfo GetterDialect] {getterOpCode : GetterDialect}
+    {op' : OperationPtr} :
+    op'.getProperties!
+      (Rewriter.setProperties ctx op opCode newProps opIn hprop)
+      getterOpCode =
     if op' = op then
-      if h : (getterOpCode : OpInfo) = opCode then
-        HasDialect.toDialectProperties getterOpCode (h ▸ newProps)
-      else default
+      if h : ofDialect OpInfo opCode = ofDialect OpInfo getterOpCode then
+        HasDialect.toDialectProperties getterOpCode
+          (h ▸ HasDialect.ofDialectProperties OpInfo opCode newProps)
+      else
+        default
     else
       op'.getProperties! ctx getterOpCode := by
   grind
 
 @[simp, grind =]
 theorem OperationPtr.getNumResults!_setProperties {op' : OperationPtr} :
-    op'.getNumResults! (Rewriter.setProperties ctx op newProps opIn) =
+    op'.getNumResults! (Rewriter.setProperties ctx op opCode newProps opIn) =
     op'.getNumResults! ctx := by
   grind
 
 @[simp, grind =]
 theorem OpResultPtr.get!_setProperties {opResult : OpResultPtr} :
-    opResult.get! (Rewriter.setProperties ctx op newProps opIn) =
+    opResult.get! (Rewriter.setProperties ctx op opCode newProps opIn) =
     opResult.get! ctx := by
   grind
 
 @[simp, grind =]
 theorem OperationPtr.getNumOperands!_setProperties {op' : OperationPtr} :
-    op'.getNumOperands! (Rewriter.setProperties ctx op newProps opIn) =
+    op'.getNumOperands! (Rewriter.setProperties ctx op opCode newProps opIn) =
     op'.getNumOperands! ctx := by
   grind
 
 @[simp, grind =]
 theorem OpOperandPtr.get!_setProperties {opOperand : OpOperandPtr} :
-    opOperand.get! (Rewriter.setProperties ctx op newProps opIn) =
+    opOperand.get! (Rewriter.setProperties ctx op opCode newProps opIn) =
     opOperand.get! ctx := by
   grind
 
 @[simp, grind =]
 theorem OperationPtr.getOperands!_setProperties {op' : OperationPtr} :
-    op'.getOperands! (Rewriter.setProperties ctx op newProps opIn) =
+    op'.getOperands! (Rewriter.setProperties ctx op opCode newProps opIn) =
     op'.getOperands! ctx := by
   grind
 
 @[simp, grind =]
 theorem OperationPtr.getNumSuccessors!_setProperties {op' : OperationPtr} :
-    op'.getNumSuccessors! (Rewriter.setProperties ctx op newProps opIn) =
+    op'.getNumSuccessors! (Rewriter.setProperties ctx op opCode newProps opIn) =
     op'.getNumSuccessors! ctx := by
   grind
 
 @[simp, grind =]
 theorem BlockOperandPtr.get!_setProperties {blockOperand : BlockOperandPtr} :
-    blockOperand.get! (Rewriter.setProperties ctx op newProps opIn) =
+    blockOperand.get! (Rewriter.setProperties ctx op opCode newProps opIn) =
     blockOperand.get! ctx := by
   grind
 
 @[simp, grind =]
 theorem OperationPtr.getSuccessor!_setProperties {op' : OperationPtr} :
-    op'.getSuccessor! (Rewriter.setProperties ctx op newProps opIn) index =
+    op'.getSuccessor! (Rewriter.setProperties ctx op opCode newProps opIn) index =
     op'.getSuccessor! ctx index := by
   grind [OperationPtr.getSuccessor!_def]
 
 @[simp, grind =]
 theorem OperationPtr.getSuccessors!_setProperties {op' : OperationPtr} :
-    op'.getSuccessors! (Rewriter.setProperties ctx op newProps opIn) =
+    op'.getSuccessors! (Rewriter.setProperties ctx op opCode newProps opIn) =
     op'.getSuccessors! ctx := by
   grind [OperationPtr.getSuccessors!_def]
 
 @[simp, grind =]
 theorem OperationPtr.getNumRegions!_setProperties {op' : OperationPtr} :
-    op'.getNumRegions! (Rewriter.setProperties ctx op newProps opIn) =
+    op'.getNumRegions! (Rewriter.setProperties ctx op opCode newProps opIn) =
     op'.getNumRegions! ctx := by
   grind [OperationPtr.getSuccessors!_def]
 
 @[simp, grind =]
 theorem OperationPtr.getRegion!_setProperties {op' : OperationPtr} :
-    op'.getRegion! (Rewriter.setProperties ctx op newProps opIn) index =
+    op'.getRegion! (Rewriter.setProperties ctx op opCode newProps opIn) index =
     op'.getRegion! ctx index := by
   grind [OperationPtr.getSuccessors!_def]
 
 @[simp, grind =]
 theorem BlockOperandPtrPtr.get!_setProperties {blockOperandPtr : BlockOperandPtrPtr} :
-    blockOperandPtr.get!  (Rewriter.setProperties ctx op newProps opIn) =
+    blockOperandPtr.get!  (Rewriter.setProperties ctx op opCode newProps opIn) =
     blockOperandPtr.get! ctx := by
   grind
 
 @[simp, grind =]
 theorem BlockPtr.getNumArguments!_setProperties {block : BlockPtr} :
-    block.getNumArguments! (Rewriter.setProperties ctx op newProps opIn) =
+    block.getNumArguments! (Rewriter.setProperties ctx op opCode newProps opIn) =
     block.getNumArguments! ctx := by
   grind
 
 @[simp, grind =]
 theorem BlockArgumentPtr.get!_setProperties {blockArgument : BlockArgumentPtr} :
-    blockArgument.get!  (Rewriter.setProperties ctx op newProps opIn) =
+    blockArgument.get!  (Rewriter.setProperties ctx op opCode newProps opIn) =
     blockArgument.get! ctx := by
   grind
 
 @[simp, grind =]
 theorem RegionPtr.get!_setProperties {region : RegionPtr} :
-    region.get! (Rewriter.setProperties ctx op newProps opIn) =
+    region.get! (Rewriter.setProperties ctx op opCode newProps opIn) =
     region.get! ctx := by
   grind
 
 @[simp, grind =]
 theorem RegionPtr.firstBlock!_setProperties {region : RegionPtr} :
-    (region.get! (Rewriter.setProperties ctx op newProps opIn)).firstBlock =
+    (region.get! (Rewriter.setProperties ctx op opCode newProps opIn)).firstBlock =
     (region.get! ctx).firstBlock := by
   grind
 
 @[simp, grind =]
 theorem RegionPtr.lastBlock!_setProperties {region : RegionPtr} :
-    (region.get! (Rewriter.setProperties ctx op newProps opIn)).lastBlock =
+    (region.get! (Rewriter.setProperties ctx op opCode newProps opIn)).lastBlock =
     (region.get! ctx).lastBlock := by
   grind
 
 @[simp, grind =]
 theorem RegionPtr.parent!_setProperties {region : RegionPtr} :
-    (region.get! (Rewriter.setProperties ctx op newProps opIn)).parent =
+    (region.get! (Rewriter.setProperties ctx op opCode newProps opIn)).parent =
     (region.get! ctx).parent := by
   grind
 
 @[simp, grind =]
 theorem ValuePtr.getFirstUse!_setProperties {value : ValuePtr} :
-    value.getFirstUse! (Rewriter.setProperties ctx op newProps opIn)  =
+    value.getFirstUse! (Rewriter.setProperties ctx op opCode newProps opIn)  =
     value.getFirstUse! ctx := by
   grind
 
 @[simp, grind =]
 theorem ValuePtr.getType!_setProperties {value : ValuePtr} :
-    value.getType! (Rewriter.setProperties ctx op newProps opIn)  =
+    value.getType! (Rewriter.setProperties ctx op opCode newProps opIn)  =
     value.getType! ctx := by
   grind
 
 @[simp, grind =]
 theorem OpOperandPtrPtr.get!_setProperties {opOperandPtr : OpOperandPtrPtr} :
-    opOperandPtr.get! (Rewriter.setProperties ctx op newProps opIn) =
+    opOperandPtr.get! (Rewriter.setProperties ctx op opCode newProps opIn) =
     opOperandPtr.get! ctx := by
   grind
 
