Veir/Rewriter/WellFormed/Operation.lean
@@ -311,11 +311,14 @@ end setAttributes
 
 section setProperties
 
-theorem OperationPtr.setProperties_WellFormed {opCode : OpInfo} (ctx: IRContext OpInfo)
+variable {Dialect : Type} [HasDialectOpInfo Dialect] [HasDialect OpInfo Dialect]
+variable {opCode : Dialect} {newProps : HasDialectOpInfo.propertiesOf opCode}
+
+theorem OperationPtr.setProperties_WellFormed (ctx: IRContext OpInfo)
   (op: OperationPtr) (hctx : ctx.WellFormed) (hop : op.InBounds ctx)
   (hprop : op.getOpType! ctx = opCode := by grind)
-  (newProperties: HasOpInfo.propertiesOf opCode) :
-  (op.setProperties ctx newProperties hop hprop).WellFormed := by
+  (newProperties: HasDialectOpInfo.propertiesOf opCode) :
+  (op.setProperties ctx opCode newProperties hop hprop).WellFormed := by
   have ⟨h₁, h₂, h₃, h₄, h₅, h₆, h₇, h₈⟩ := hctx
   constructor
   · grind
@@ -323,49 +326,51 @@ theorem OperationPtr.setProperties_WellFormed {opCode : OpInfo} (ctx: IRContext 
     have ⟨array, harray⟩ := h₂ val (by grind)
     exists array
     simp only [Std.ExtHashSet.filter_empty] at harray ⊢
-    apply ValuePtr.DefUse.unchanged harray (ctx' := op.setProperties ctx newProperties hop hprop) <;> grind
+    apply ValuePtr.DefUse.unchanged harray (ctx' := op.setProperties ctx opCode newProperties hop hprop) <;> grind
   · intro blk hblk
     have ⟨array, harray⟩ := h₃ blk (by grind)
     exists array
     simp only [Std.ExtHashSet.filter_empty] at harray ⊢
-    apply BlockPtr.DefUse.unchanged harray (ctx' := op.setProperties ctx newProperties hop hprop) <;> grind
+    apply BlockPtr.DefUse.unchanged harray (ctx' := op.setProperties ctx opCode newProperties hop hprop) <;> grind
   · intro blk hblk
     have ⟨array, harray⟩ := h₄ blk (by grind)
     exists array
-    apply BlockPtr.OpChain_unchanged harray (ctx' := op.setProperties ctx newProperties hop hprop) <;> grind
+    apply BlockPtr.OpChain_unchanged harray (ctx' := op.setProperties ctx opCode newProperties hop hprop) <;> grind
   · intro reg hreg
     have ⟨array, harray⟩ := h₅ reg (by grind)
     exists array
-    apply RegionPtr.blockChain_unchanged harray (ctx' := op.setProperties ctx newProperties hop hprop) <;> grind
+    apply RegionPtr.blockChain_unchanged harray (ctx' := op.setProperties ctx opCode newProperties hop hprop) <;> grind
   · intro op' hop'
     have h_wf := h₆ op' (by grind)
-    apply OperationPtr.WellFormed_unchanged h_wf (ctx' := op.setProperties ctx newProperties hop hprop) <;> grind
+    apply OperationPtr.WellFormed_unchanged h_wf (ctx' := op.setProperties ctx opCode newProperties hop hprop) <;> grind
   · intro blk hblk
     have h_wf := h₇ blk (by grind)
-    apply BlockPtr.WellFormed_unchanged h_wf (ctx' := op.setProperties ctx newProperties hop hprop) <;> grind
+    apply BlockPtr.WellFormed_unchanged h_wf (ctx' := op.setProperties ctx opCode newProperties hop hprop) <;> grind
   · intro reg hreg
     have h_wf := h₈ reg (by grind)
-    apply RegionPtr.WellFormed_unchanged h_wf (ctx' := op.setProperties ctx newProperties hop hprop) <;> grind
+    apply RegionPtr.WellFormed_unchanged h_wf (ctx' := op.setProperties ctx opCode newProperties hop hprop) <;> grind
 
 theorem BlockPtr.opChain_OperationPtr_setProperties
     (hWf : BlockPtr.OpChain block' ctx array)
     {op : OperationPtr} (hop : op.InBounds ctx)
-    {opCode : OpInfo} (newProps : HasOpInfo.propertiesOf opCode)
+    (newProps : HasDialectOpInfo.propertiesOf opCode)
     (hprop : op.getOpType! ctx = opCode := by grind) :
-    BlockPtr.OpChain block' (op.setProperties ctx newProps hop hprop) array := by
+    BlockPtr.OpChain block' (op.setProperties ctx opCode newProps hop hprop) array := by
   apply BlockPtr.OpChain_unchanged (ctx := ctx) <;> grind
 
 @[grind =]
 theorem BlockPtr.operationList_operationPtr_setProperties
     (hctx : ctx.WellFormed) :
-    BlockPtr.operationList block' (OperationPtr.setProperties op ctx newProps hop hprop) ctx' blockInBounds' =
+    BlockPtr.operationList block' (OperationPtr.setProperties op ctx opCode newProps hop hprop) ctx' blockInBounds' =
     BlockPtr.operationList block' ctx hctx (by grind) := by
   simp only [← BlockPtr.operationList_iff_BlockPtr_OpChain]
   grind [BlockPtr.opChain_OperationPtr_setProperties]
 
 theorem Rewriter.setProperties_WellFormed
+    {op : OperationPtr} {hop : op.InBounds ctx}
+    {hprop : op.getOpType! ctx = opCode}
     (hctx : ctx.WellFormed) :
-    (Rewriter.setProperties ctx op newProps hop hprop).WellFormed := by
+    (Rewriter.setProperties ctx op opCode newProps hop hprop).WellFormed := by
    grind [setProperties, OperationPtr.setProperties_WellFormed]
 
 end setProperties
